theories/LambdaANF/LambdaBoxLocal_to_LambdaANF_correct.v
@@ -539,71 +539,11 @@ Section Correct.
       - destruct n; simpl in *.
         + inv Hnth1. inv Hnth2. destructAll. eauto.
         + eauto.
-    Qed. 
-
-    Lemma preord_var_env_extend_neq_l PostG (rho1 rho2 : eval.env) (k : nat) (x1 y1 y2 : var)
-          (v1 : cps.val) :
-        preord_var_env cenv PostG k rho1 rho2 y1 y2 ->
-        y1 <> x1 ->
-        preord_var_env cenv PostG k (M.set x1 v1 rho1) rho2 y1 y2.
-    Proof.
-      intros Hval Hneq x' Hget.
-      rewrite M.gso in *; eauto.
-    Qed.
-
-    Lemma preord_var_env_extend_neq_r PostG (rho1 rho2 : eval.env) (k : nat) (x1 y1 y2 : var)
-          (v1 : cps.val) :
-      preord_var_env cenv PostG k rho1 rho2 y1 y2 ->
-      y2 <> x1 ->
-      preord_var_env cenv PostG k rho1 (M.set x1 v1 rho2) y1 y2.
-    Proof.
-      intros Hval Hneq x' Hget.
-      rewrite M.gso in *; eauto.
-    Qed.
-
-    Lemma preord_var_env_get :
-      forall PostG (rho1 rho2 : eval.env) (k : nat) (x1 x2 : var) (v1 v2 : cps.val),
-        preord_val cenv PostG k v1 v2 ->
-        M.get x1 rho1 = Some v1 ->
-        M.get x2 rho2 = Some v2 ->        
-        preord_var_env cenv PostG k rho1 rho2 x1 x2.
-    Proof.
-      intros rho1 rho2 k x1 x2 v1 v2 Hval Hget1 Hget2 x' v' Hget.
-      repeat subst_exp. eauto. 
-    Qed.
-
-    Lemma preord_var_env_get_list :
-      forall PostG (rho1 rho2 : eval.env) (k : nat) (xs1 xs2 : list var) (vs1 vs2 : list cps.val),
-        Forall2 (preord_val cenv PostG k) vs1 vs2 ->
-        get_list xs1 rho1 = Some vs1 ->
-        get_list xs2 rho2 = Some vs2 ->        
-        Forall2 (preord_var_env cenv PostG k rho1 rho2) xs1 xs2.
-    Proof.
-      intros PG rho1 rho2 k xs1.
-      revert rho1 rho2. induction xs1; intros rho1 rho2 xs2 vs1 vs2 Hall Hget1 Hget2.
-      - simpl in Hget1. inv Hget1. inv Hall.
-        destruct xs2. now constructor.
-        simpl in *. destruct (rho2 ! v); try congruence.
-        destruct (get_list xs2 rho2); congruence.
-      - simpl in Hget1.
-         destruct (rho1 ! a) eqn:Hget; try congruence.
-         destruct (get_list xs1 rho1) eqn:Hgetl; try congruence.
-         inv Hget1.
-         inv Hall.
-         destruct xs2. now inv Hget2. simpl in *.
-         destruct (rho2 ! v0) eqn:Hget'; try congruence.
-         destruct (get_list xs2 rho2) eqn:Hgetl'; try congruence.
-         inv Hget2.
-         constructor; eauto.
-
-         eapply preord_var_env_get; eauto.
     Qed.
 
     
-
     Definition one_step : @PostT nat unit :=
       fun '(e1, r1, f1, t1) '(e2, r2, f2, t2) => (f1 + 1)%nat = f2.
-
 
     Lemma preord_exp_Efun_red k e B rho :          
       preord_exp cenv one_step eq_fuel k (e, def_funs B B rho rho) (Efun B e, rho).
